Nemonuri/Executions/ExecutionFragment/Expr/Raw.lean
@@ -6,6 +6,8 @@ public import Nemonuri.Executions.ExecutionFragment.Raw
 
 namespace Nemonuri.TransitionSystem.ExecutionFragment
 
+open Nemonuri.HasLabel
+
 inductive ExprRaw (ts: TransitionSystem) where
   | finite1 (total: ts.FiniteExecutionFragmentRaw)
   | finite2 (pre: ts.FiniteExecutionFragmentRaw) (post: ts.FiniteExecutionFragmentRaw)
@@ -15,19 +17,123 @@ namespace ExprRaw
 
 variable {ts: TransitionSystem}
 
+inductive Label where
+  | finite1
+  | finite2
+  | infinite1
+  deriving DecidableEq, Repr, Fintype
+
+def toLabel : ExprRaw ts → Label
+  | .finite1 _ => .finite1
+  | .finite2 _ _ => .finite2
+  | .infinite1 _ => .infinite1
+
+@[defeq, simp]
+theorem finite1_toLabel {x} : (@ExprRaw.finite1 ts x).toLabel = .finite1 := rfl
+
+@[defeq, simp]
+theorem finite2_toLabel {x1 x2} : (@ExprRaw.finite2 ts x1 x2).toLabel = .finite2 := rfl
+
+@[defeq, simp]
+theorem infinite1_toLabel {x} : (@ExprRaw.infinite1 ts x).toLabel = .infinite1 := rfl
+
+instance : HasLabel Label (ExprRaw ts) := ⟨toLabel⟩
+
+
+def Label.toSeqLabel : Label → Sequence.Label
+  | .finite1 | .finite2 => .finite
+  | .infinite1 => .infinite
+
+def toSeqLabel (raw: ExprRaw ts) : Sequence.Label := raw.toLabel.toSeqLabel
+
+@[defeq, simp]
+theorem finite1_toSeqLabel {x} : (@ExprRaw.finite1 ts x).toSeqLabel = .finite := rfl
+
+@[defeq, simp]
+theorem finite2_toSeqLabel {x1 x2} : (@ExprRaw.finite2 ts x1 x2).toSeqLabel = .finite := rfl
+
+@[defeq, simp]
+theorem infinite1_toSeqLabel {x} : (@ExprRaw.infinite1 ts x).toSeqLabel = .infinite := rfl
+
+instance : HasLabel Sequence.Label (ExprRaw ts) := ⟨toSeqLabel⟩
+
+
+
+
 def singleState (s: ts.S) : ExprRaw ts := .finite1 (.singleState s)
 
+section SingleState
+
+variable {s: ts.S}
+
+@[defeq, simp]
+theorem singleState_toLabel : (singleState s).toLabel = .finite1 := rfl
+
+@[defeq, simp]
+theorem singleState_toSeqLabel : (singleState s).toSeqLabel = .finite := rfl
+
+end SingleState
+
+
 def ellipsis : ExprRaw ts := .infinite1 (⟨[],[]⟩)
+
+section Ellipsis
+
+@[defeq, simp]
+theorem ellipsis_toLabel : (@ellipsis ts).toLabel = .infinite1 := rfl
+
+@[defeq, simp]
+theorem ellipsis_toSeqLabel : (@ellipsis ts).toSeqLabel = .infinite := rfl
+
+end Ellipsis
+
 
 def consEllipsis : ExprRaw ts → ExprRaw ts
   | .finite1 total => .finite2 (⟨[],[]⟩) total
   | x => x
+
+theorem consEllipsis_preserves_seqLabel : HasLabel.Preserves Sequence.Label (@consEllipsis ts) := by
+  apply Preserves.mk _ ?_
+  intro x
+  cases x <;> rfl
+
 
 def stepL (tail: ExprRaw ts) (s: ts.S) (a: ts.Act) : ExprRaw ts :=
   match tail with
   | .finite1 total => .finite1 (total.stepL s a)
   | .finite2 pre post => .finite2 (pre.stepL s a) post
   | .infinite1 pre => .infinite1 (pre.stepL s a)
+
+theorem stepL_preserves_label {s a} : HasLabel.Preserves Label (@stepL ts · s a) := by
+  apply Preserves.mk _ ?_
+  intro x
+  cases x <;> rfl
+
+theorem stepL_preserves_seqLabel {s a} : HasLabel.Preserves Sequence.Label (@stepL ts · s a) := by
+  apply Preserves.mk _ ?_
+  intro x
+  cases x <;> rfl
+
+
+def stepL' (s: ts.S) (a: ts.Act) (tail: ExprRaw ts) : ExprRaw ts := tail.stepL s a
+
+@[defeq]
+theorem stepL_eq_stepL' {tail s a} : (@stepL ts tail s a) = (@stepL' ts s a tail) := rfl
+
+theorem stepL'_preserves_label {s a} : HasLabel.Preserves Label (@stepL' ts s a) := @stepL_preserves_label ts s a
+
+theorem stepL'_preserves_seqLabel {s a} : HasLabel.Preserves Sequence.Label (@stepL' ts s a) := @stepL_preserves_seqLabel ts s a
+
+
+--def pre :
+
+section
+
+variable {tail: ExprRaw ts} {s: ts.S} {a: ts.Act}
+
+--theorem stepL_finite1 (req: tail.toSeqLabel = .finite) : (tail.stepL s a)
+
+end
 
 instance : Coe ts.S (ExprRaw ts) := ⟨singleState⟩
 
