Nemonuri.lean
@@ -1,5 +1,6 @@
 module
 
+public import Nemonuri.HasLabel
 public import Nemonuri.Sequence
 public import Nemonuri.ModelChecking
 public import Nemonuri.PropositionalLogics
