Nemonuri/Examples/BeverageVendingMachineOfExecution.lean
@@ -3,6 +3,7 @@ module
 
 public import Nemonuri.Examples.BeverageVendingMachine
 public import Nemonuri.Executions.ExecutionFragment.Expr
+public import Nemonuri.Executions.ExecutionFragment.Maximal
 
 /-!
 
@@ -25,14 +26,53 @@ open ExecutionFragment Expr
 def ρ₁ := 𝐸𝑥𝑒𝑐{ts}⸨ &(.pay) ─⌞.insert_coin⌟→ &(.select) ─⌞.τ⌟→ &(.soda) ─⌞.get_soda⌟→ &(.pay)
                     ─⌞.insert_coin⌟→ &(.select) ─⌞.τ⌟→ &(.soda) ─⌞.get_soda⌟→ ... ⸩
 
-/-
-theorem ρ₁_nonempty : ρ₁.Nonempty := by
-  rw [Set.nonempty_def]
--/
-  --dsimp [ρ₁]
-  --dsimp [ExprRaw.EvalToSet]
+def ρ₂ := 𝐸𝑥𝑒𝑐{ts}⸨ &(.select)─⌞.τ⌟→ &(.soda)─⌞.get_soda⌟→ &(.pay)─⌞.insert_coin⌟→ &(.select)─⌞.τ⌟→ &(.beer)─⌞.get_beer⌟→ ...⸩
+
+def ϱ := 𝐸𝑥𝑒𝑐{ts}⸨ &(.pay) ─⌞.insert_coin⌟→ &(.select)─⌞.τ⌟→ &(.soda)─⌞.get_soda⌟→ &(.pay)
+                    ─⌞.insert_coin⌟→ &(.select)─⌞.τ⌟→ State.soda ⸩
+
+/-! Execution fragments `ρ₁` and `ϱ` are initial, but `ρ₂` is not. -/
+
+#print ExprRaw.Mem.infinite1
+#print HasLabel.toLabel
+
+theorem ρ₁_initial (x: ρ₁) : x.val.IsInitial := by
+  revert x
+  simp only [Subtype.forall]
+  intro x lm1
+  dsimp [ρ₁] at lm1
+  have lm2 := ExprRaw.EvalToSet.mem_imp_isExecutionFragment _ _ lm1
+  dsimp [ExecutionFragmentRaw.IsInitial]
+  exists lm2
+  dsimp [ExecutionFragment.IsInitial]
+  simp only [Set.mem_singleton_iff]
+  dsimp only [ExecutionFragment.state0, ExecutionFragment.states]
+  dsimp [ExprRaw.EvalToSet] at lm1
+  cases x
+  · refine absurd lm1 ?_
+    refine ExprRaw.mem_not_finite_infinite ?_ ?_
+    · dsimp
+    · simp only [ExprRaw.stepL_eq_stepL']
+      conv => lhs; change (HasLabel.toLabel (_: ExprRaw ts): Sequence.Label)
+      simp only [ExprRaw.stepL'_preserves_seqLabel, ← HasLabel.Preserves.apply]
+      rfl
+  · sorry
 
 
+
+
+      --have lm3 s a := HasLabel.LabelHom.coe_mk _ (@ExprRaw.stepL'_preserves_seqLabel ts s a)
+      --conv => lhs; arg 1; dsimp [ExprRaw.stepL]
+
+
+
+
+      --have lm3 := HasLabel.LabelHom.coe_mk _ ExprRaw.stepL_preserves_seqLabel
+
+  --have lm1 := x.property
+  --have lm2 :=
+  --dsimp [ExecutionFragment.IsInitial]
+  --simp only [Set.mem_singleton_iff]
 
 
 end Examples.Executions
