Nemonuri/Executions/ExecutionFragment/Expr/Notation.lean
@@ -36,6 +36,7 @@ macro_rules
 
 syntax:100 exec_expr:99 "─⌞" term "⌟→" exec_expr:100 : exec_expr
 
+
 macro_rules
   | `(exec_expr| $s:exec_expr ─⌞ $a:term ⌟→ $tail:exec_expr ) => do `(ExprRaw.stepL $(.mk (← pure tail)) $(.mk (← pure s)) $a)
 
