Nemonuri/Executions/FiniteExecutionFragment/Prefix.lean
@@ -1,0 +1,36 @@
+module
+
+public import Nemonuri.Executions.FiniteExecutionFragment.Basic
+
+@[expose] public section
+
+namespace Nemonuri.TransitionSystem
+
+namespace FiniteExecutionFragmentRaw
+
+variable {ts: TransitionSystem}
+
+inductive IsPrefixFragment : ts.FiniteExecutionFragmentRaw → Prop where
+  | intro (states: List ts.S) (actions: List ts.Act) (stateLast: ts.S)
+          (req: ts.IsFiniteExecutionFragment ⟨states ++ [stateLast], actions⟩)
+          : IsPrefixFragment ⟨states ++ [stateLast], actions⟩
+
+inductive IsSuffixFragment : ts.FiniteExecutionFragmentRaw → Prop where
+  | intro (states: List ts.S) (actions: List ts.Act) (state0: ts.S)
+          (req: ts.IsFiniteExecutionFragment ⟨state0 :: states, actions⟩)
+          : IsSuffixFragment ⟨state0 :: states, actions⟩
+
+
+structure PrefixFragment (ts: TransitionSystem) where
+  raw: ts.FiniteExecutionFragmentRaw
+  is_valid: IsPrefixFragment raw
+
+structure SuffixFragment (ts: TransitionSystem) where
+  raw: ts.FiniteExecutionFragmentRaw
+  is_valid: IsSuffixFragment raw
+
+end FiniteExecutionFragmentRaw
+
+end Nemonuri.TransitionSystem
+
+end
