Nemonuri/HasLabel.lean
@@ -1,0 +1,159 @@
+module
+
+public import Mathlib.Data.Fintype.Basic
+public import Mathlib.Data.FunLike.Basic
+
+
+@[expose] public section
+
+namespace Nemonuri
+
+class HasLabel (Label: Type _) [DecidableEq Label] [Fintype Label] (T: Type _)  where
+  toLabel (t: T) : Label
+
+namespace HasLabel
+
+section Definition
+
+variable (Label: Type _) [DecidableEq Label] [Fintype Label] {T1: Type _} [HasLabel Label T1] {T2: Type _} [HasLabel Label T2]
+
+def Preserves (f: (_: T1) → T2) : Prop := ∀ ⦃x: T1⦄, (toLabel x : Label) = (toLabel (f x))
+
+structure LabelHom (T1: Type _) [HasLabel Label T1] (T2: Type _) [HasLabel Label T2] where
+  toFun: T1 → T2
+  preserves: Preserves Label toFun
+
+class IsLabelHomLike
+  (F: Type _) (Label T1 T2: outParam (Type _))
+  [DecidableEq Label] [Fintype Label] [HasLabel Label T1] [HasLabel Label T2] [FunLike F T1 T2] : Prop where
+  preserves (f: F) : Preserves Label (f: T1 → T2)
+
+end Definition
+
+variable {Label: Type _} [DecidableEq Label] [Fintype Label]
+         {T1: Type _} [HasLabel Label T1] {T2: Type _} [HasLabel Label T2] {T3: Type _} [HasLabel Label T3]
+
+theorem preserves_def {f: T1 → T2} : Preserves Label f ↔ ∀(x: T1), (toLabel x : Label) = (toLabel (f x)) := Iff.rfl
+
+namespace Preserves
+
+theorem mk (f: T1 → T2) (req: ∀(x: T1), (toLabel x : Label) = (toLabel (f x))) : Preserves Label f := req
+
+theorem apply (f: T1 → T2) (h: Preserves Label f) (x: T1) : (toLabel x : Label) = (toLabel (f x)) := @h x
+
+theorem comp {fl: T2 → T3} {fr: T1 → T2} (h1: Preserves Label fl) (h2: Preserves Label fr) : Preserves Label (fl ∘ fr) := by
+  revert h1 h2; dsimp [Preserves]
+  intro h1 h2 x
+  specialize @h2 x
+  specialize @h1 (fr x)
+  exact Eq.trans h2 h1
+
+end Preserves
+
+
+
+namespace LabelHom
+
+
+instance toFunlike : FunLike (LabelHom Label T1 T2) T1 T2 where
+  coe lh := lh.toFun
+  coe_injective lh1 lh2 := by cases lh1; cases lh2; dsimp; intro lm1; subst lm1; rfl
+
+instance is_labelHomLike : IsLabelHomLike (LabelHom Label T1 T2) Label T1 T2 where
+  preserves lh := lh.preserves
+
+
+
+@[defeq, simp]
+theorem coe_mk (f: T1 → T2) (req: Preserves Label f) : ((LabelHom.mk f req): T1 → T2) = f := rfl
+
+@[defeq, simp]
+theorem toFun_eq_coe (f: LabelHom Label T1 T2) : f.toFun = f := rfl
+
+@[ext]
+theorem ext ⦃f1 f2: LabelHom Label T1 T2⦄ (h: ∀x, f1 x = f2 x) : f1 = f2 := DFunLike.ext _ _ h
+
+@[defeq, simp]
+theorem mk_coe (f: LabelHom Label T1 T2) (req: Preserves Label f) : (LabelHom.mk f req) = f :=
+  LabelHom.ext (fun _ => rfl)
+
+protected def copy (f1: LabelHom Label T1 T2) (f2: T1 → T2) (h: f2 = f1) : LabelHom Label T1 T2 where
+  toFun := f2
+  preserves := h.symm ▸ f1.preserves
+
+section
+
+omit [HasLabel Label T1] [HasLabel Label T2]
+
+@[simp]
+theorem coe_copy {_: HasLabel Label T1} {_: HasLabel Label T2} (f1: LabelHom Label T1 T2) (f2: T1 → T2) (h: f2 = f1)
+  : (f1.copy f2 h) = f2 :=
+  rfl
+
+theorem coe_copy_eq {_: HasLabel Label T1} {_: HasLabel Label T2} (f1: LabelHom Label T1 T2) (f2: T1 → T2) (h: f2 = f1)
+  : f1.copy f2 h = f1 :=
+  DFunLike.ext' h
+
+end
+
+@[simps, implicit_reducible]
+def id (Label: Type _) [DecidableEq Label] [Fintype Label] (T: Type _) [HasLabel Label T] : LabelHom Label T T where
+  toFun x := x
+  preserves _ := rfl
+
+@[simp]
+theorem coe_id : (LabelHom.id Label T1 : T1 → T1) = _root_.id := rfl
+
+
+@[implicit_reducible]
+def comp (lhl: LabelHom Label T2 T3) (lhr: LabelHom Label T1 T2) : LabelHom Label T1 T3 where
+  toFun x := lhl (lhr x)
+  preserves := by
+    refine Preserves.comp ?_ ?_
+    · exact lhl.preserves
+    · exact lhr.preserves
+
+@[defeq]
+theorem coe_comp (lhl: LabelHom Label T2 T3) (lhr: LabelHom Label T1 T2)
+  : ↑(lhl.comp lhr) = lhl ∘ lhr :=
+  rfl
+
+@[defeq]
+theorem comp_apply (lhl: LabelHom Label T2 T3) (lhr: LabelHom Label T1 T2) (x: T1) : lhl.comp lhr x = lhl (lhr x) := rfl
+
+@[defeq]
+theorem comp_assoc {T4: Type _} [HasLabel Label T4] (lh1: LabelHom Label T1 T2) (lh2: LabelHom Label T2 T3) (lh3: LabelHom Label T3 T4)
+  : (lh3.comp lh2).comp lh1 = lh3.comp (lh2.comp lh1) := rfl
+
+@[defeq, simp]
+theorem comp_id (f: LabelHom Label T1 T2) : f.comp (LabelHom.id Label T1) = f := LabelHom.ext (fun _ => rfl)
+
+@[defeq, simp]
+theorem id_comp (f: LabelHom Label T1 T2) : (LabelHom.id Label T2).comp f = f := LabelHom.ext (fun _ => rfl)
+
+end LabelHom
+
+
+namespace IsLabelHomLike
+
+variable {F: Type _} {T1 T2 Label: outParam (Type _)} [DecidableEq Label] [Fintype Label] [HasLabel Label T1] [HasLabel Label T2] [FunLike F T1 T2]
+
+@[coe]
+def toLabelHom [IsLabelHomLike F Label T1 T2] (f: F) : LabelHom Label T1 T2 where
+  toFun := f
+  preserves := IsLabelHomLike.preserves f
+
+instance [IsLabelHomLike F Label T1 T2] : CoeHead F (LabelHom Label T1 T2) := ⟨toLabelHom⟩
+
+@[defeq, simp]
+theorem coe_coe [IsLabelHomLike F Label T1 T2] (f: F) : ((f: LabelHom Label T1 T2): T1 → T2) = f := rfl
+
+
+end IsLabelHomLike
+
+
+end HasLabel
+
+end Nemonuri
+
+end
